src/ByteStringHeap.v
@@ -1,22 +1,10 @@
 Require Import
-  Coq.Lists.List
-  Coq.Arith.Arith
-  Coq.NArith.NArith
-  Fiat.ADT
-  Fiat.ADTNotation
-  Fiat.ADTRefinement
-  Fiat.ADTRefinement.BuildADTRefinements
-  ByteString.ADTInduction
-  ByteString.BindDep
-  ByteString.ByteString
-  ByteString.Memory
-  ByteString.Heap
-  ByteString.Nomega
-  ByteString.Relations
   ByteString.Tactics
-  ByteString.TupleEnsembles
-  ByteString.Same_set
-  ByteString.Within
+  ByteString.Memory
+  ByteString.Nomega
+  ByteString.Heap
+  ByteString.ByteString
+  ByteString.Fiat
   Coq.FSets.FMapFacts
   Coq.Structures.DecidableTypeEx.
 
@@ -27,34 +15,12 @@ Open Scope N_scope.
 Module ByteStringHeap (M : WSfun N_as_DT).
 
 Module Import HeapCanonical := HeapCanonical M.
-Import HeapADT.
+
 Import HeapADT.Heap.
 Import HeapADT.Heap.FMapExt.
-Import HeapADT.Heap.FMapExt.P.
-Import HeapADT.Heap.FMapExt.F.
-
-Definition HSpec := projT1 HeapSpecADT.
-
-Definition memcpy' (r : Rep HSpec) (addr : Ptr) (addr2 : Ptr) (len : Size) :
-  Comp (Rep HSpec * unit) :=
-  Eval simpl in callMeth HSpec memcpyS r addr addr2 len.
-
-Definition alloc' (r : Rep HSpec) (len : Size | 0 < len) :
-  Comp (Rep HSpec * Ptr) :=
-  Eval simpl in callMeth HSpec allocS r len.
-
-Definition free' (r : Rep HSpec) (addr : Ptr) : Comp (Rep HSpec * unit) :=
-  Eval simpl in callMeth HSpec freeS r addr.
-
-Definition peek' (r : Rep HSpec) (addr : Ptr) : Comp (Rep HSpec * Word) :=
-  Eval simpl in callMeth HSpec peekS r addr.
-
-Definition poke' (r : Rep HSpec) (addr : Ptr) (w : Word) :
-  Comp (Rep HSpec * unit) :=
-  Eval simpl in callMeth HSpec pokeS r addr w.
 
 Record PS := makePS {
-  psHeap : Rep HSpec;
+  psHeap : Rep HeapSpec;
 
   psBuffer : Ptr;
   psBufLen : Size;
@@ -74,7 +40,7 @@ Program Definition make_room_by_shifting_up (r : PS) (n : N | 0 < n) :
   (* We could maybe be smarter by shifting the block so it sits mid-way within
      the buffer. *)
   Comp PS :=
-  res <- memcpy' (psHeap r) (psBuffer r) (psBuffer r + n) (psLength r);
+  res <- memcpy (psHeap r) (psBuffer r) (psBuffer r + n) (psLength r);
   ret {| psHeap   := fst res
        ; psBuffer := psBuffer r
        ; psBufLen := psBufLen r
@@ -85,9 +51,9 @@ Program Definition make_room_by_growing_buffer (r : PS) (n : N | 0 < n) :
   Comp PS :=
   (* We can make a trade-off here by allocating extra bytes in anticipation of
      future calls to [buffer_cons]. *)
-  `(h, a) <- alloc' (psHeap r) (psLength r + n);
-  `(h, _) <- memcpy' h (psBuffer r) (a + n) (psLength r);
-  `(h, _) <- free' h (psBuffer r);
+  `(h, a) <- alloc (psHeap r) (psLength r + n);
+  `(h, _) <- memcpy h (psBuffer r) (a + n) (psLength r);
+  `(h, _) <- free h (psBuffer r);
   ret {| psHeap   := h
        ; psBuffer := a
        ; psBufLen := psLength r + n
@@ -95,9 +61,9 @@ Program Definition make_room_by_growing_buffer (r : PS) (n : N | 0 < n) :
        ; psLength := psLength r + n |}.
 Obligation 1. nomega. Defined.
 
-Program Definition allocate_buffer (r : Rep HSpec) (len : N | 0 < len) :
+Program Definition allocate_buffer (r : Rep HeapSpec) (len : N | 0 < len) :
   Comp PS :=
-  `(h, a) <- alloc' r len;
+  `(h, a) <- alloc r len;
   ret {| psHeap   := h
        ; psBuffer := a
        ; psBufLen := len
@@ -105,7 +71,7 @@ Program Definition allocate_buffer (r : Rep HSpec) (len : N | 0 < len) :
        ; psLength := len |}.
 
 Definition poke_at_offset (r : PS) (d : Word) : Comp PS :=
-  res <- poke' (psHeap r) (psBuffer r + psOffset r) d;
+  res <- poke (psHeap r) (psBuffer r + psOffset r) d;
   ret {| psHeap   := fst res
        ; psBuffer := psBuffer r
        ; psBufLen := psBufLen r
@@ -133,7 +99,7 @@ Obligation 3. nomega. Defined.
 Definition buffer_uncons (r : PS) : Comp (PS * option Word) :=
   If 0 <? psLength r
   Then (
-    w <- peek' (psHeap r) (psBuffer r + psOffset r);
+    w <- peek (psHeap r) (psBuffer r + psOffset r);
     ret ({| psHeap   := psHeap r
           ; psBuffer := psBuffer r
           ; psBufLen := psBufLen r
@@ -149,11 +115,11 @@ Definition ByteString_list_AbsR (or : Rep ByteStringSpec) (nr : PS) :=
   then psOffset nr = 0 /\ psLength nr = 0
   else fits (psBuffer nr) (psBufLen nr)
             (psBuffer nr + psOffset nr) (psLength nr) /\
-       M.MapsTo (psBuffer nr) (psBufLen nr) (resvs (` (psHeap nr))) /\
+       M.MapsTo (psBuffer nr) (psBufLen nr) (resvs (psHeap nr)) /\
        (forall i x, i < psLength nr
           -> nth (N.to_nat i) or x = x
           -> M.MapsTo (psBuffer nr + psOffset nr + i) x
-                      (bytes (` (psHeap nr)))).
+                      (bytes (psHeap nr))).
 
 Ltac destruct_AbsR H :=
   let H1 := fresh "H1" in
@@ -167,167 +133,6 @@ Ltac destruct_AbsR H :=
 
 Ltac construct_AbsR := split; try split; simpl; try nomega.
 
-(*
-Ltac competing_lookups R H A1 H0 A2 :=
-  let Heqe := fresh "Heqe" in
-  destruct (A1 =? A2) eqn:Heqe;
-    [ apply Neqb_ok in Heqe; subst;
-      pose proof (allocations_functional (proj2_sig R) _ _ H _ H0);
-      subst; try nomega
-    | apply N.eqb_neq in Heqe;
-      pose proof (allocations_no_overlap (proj2_sig R) _ H _ H0 Heqe);
-      try nomega ].
-*)
-
-Ltac resolve_contention :=
-  match goal with
-  | [ H : All _ ?R, H0 : Lookup ?A ?B ?R |- _ ] => destruct (H A B)
-  end.
-
-(*
-Lemma KeepKeys_nothing : forall P m,
-  (forall a, ~ P a) -> KeepKeys P m = Empty.
-Proof.
-  intros.
-  apply Extensionality_Ensembles, Same_Same_set.
-  split; unfold KeepKeys; intros;
-  teardown; firstorder.
-Qed.
-
-Lemma KeepKeys_everything : forall (P : N -> Prop) m,
-  (forall a, P a) -> KeepKeys P m = m.
-Proof.
-  intros.
-  apply Extensionality_Ensembles, Same_Same_set.
-  split; unfold KeepKeys; intros;
-  teardown; firstorder.
-Qed.
-
-Lemma ShiftKeys_nothing : forall a b, ShiftKeys a b Empty = Empty.
-Proof.
-  intros.
-  apply Extensionality_Ensembles, Same_Same_set.
-  split; unfold ShiftKeys; intros;
-  teardown; firstorder.
-Qed.
-
-Lemma CopyBlock_nothing : forall base1 base2 addr1 addr2 blk1 blk2 len,
-  len = 0 ->
-    CopyBlock blk1 (addr1 - base1) blk2 (addr2 - base2) len = memData blk2.
-Proof.
-  intros; subst.
-  unfold CopyBlock.
-  unfold not, compose.
-  rewrite KeepKeys_everything; [|nomega].
-  rewrite KeepKeys_nothing; [|nomega].
-  rewrite ShiftKeys_nothing.
-  apply Extensionality_Ensembles.
-  apply Same_Same_set; split; intros.
-    teardown; firstorder.
-  left; assumption.
-Qed.
-*)
-
-Axiom Extensionality_FMap : forall (elt : Type) (A B : M.t elt),
-  M.Equal (elt:=elt) A B -> A = B.
-
-Lemma refine_ret_ret_fst_Equal : forall A (x z : M.t A) B (y w : B),
-  M.Equal x z -> y = w -> refine (ret (x, y)) (ret (z, w)).
-Proof.
-  intros; subst; f_equiv; f_equal.
-  apply Extensionality_FMap; assumption.
-Qed.
-
-(*
-Corollary refine_memcpy_zero heap addr1 addr2 :
-  refineEquiv (memcpy heap addr1 addr2 0) (ret (heap, tt)).
-Proof.
-  unfold memcpy; split;
-  destruct heap;
-  apply refine_ret_eq; do 3 f_equal;
-  apply Extensionality_FMap;
-  rewrite copy_bytes_zero; simpl;
-  reflexivity.
-Qed.
-
-Lemma Map_unique_is_Update heap base blk addr len f :
-  fromADT HeapSpec heap ->
-  Lookup base blk heap ->
-  fits base (memSize blk) addr len ->
-  Unique (fun a b => fits_bool a (memSize b) addr len) base heap ->
-  Same (Map (fun daddr dblk =>
-               Ifdec fits daddr (memSize dblk) addr len
-               Then f daddr dblk
-               Else dblk) heap)
-       (Update base (f base blk) heap).
-Proof.
-  intros; apply Unique_Map_Update; eauto.
-  - apply N.eq_dec.
-  - apply allocations_functional; assumption.
-  - nomega.
-Qed.
-
-Lemma refine_memcpy_existing_blocks
-      heap base1 base2 addr1 addr2 len blk1 blk2 :
-  fromADT HeapSpec heap ->
-  Lookup base1 blk1 heap ->
-  fits base1 (memSize blk1) addr1 len ->
-  Lookup base2 blk2 heap ->
-  fits base2 (memSize blk2) addr2 len ->
-  refineEquiv
-    (memcpy heap addr1 addr2 len)
-    (ret (Update base2
-            {| memSize := memSize blk2
-             ; memData :=
-                 CopyBlock blk1 (addr1 - base1)
-                           blk2 (addr2 - base2) len |} heap, tt)).
-Proof.
-  unfold memcpy, FindBlockThatFits; intro HH; intros.
-  unfold Ifdec_Then_Else at 1; simpl.
-  destruct (0 <? len) eqn:Heqe.
-    split.
-      refine pick val (Some (base1, blk1)).
-        simplify with monad laws; simpl.
-        apply refine_ret_ret_fst_Same; trivial.
-        apply Same_Same_set.
-        rewrite Map_unique_is_Update; eauto.
-          reflexivity.
-        eapply allocations_unique_fits; eauto.
-      intuition.
-    intros ??.
-    destruct_computations.
-    destruct x; try destruct p; simpl.
-      destruct H3.
-      competing_lookups (exist _ heap HH) H base1 H3 n.
-      apply eq_ret_compute; f_equal.
-      apply Extensionality_Ensembles, Same_Same_set.
-      symmetry.
-      rewrite Map_unique_is_Update;
-      [|assumption|exact H1|assumption|].
-        reflexivity.
-      eapply allocations_unique_fits; eauto.
-    clear H1.
-    resolve_contention; auto; nomega.
-  assert (len = 0) by nomega.
-  rewrite CopyBlock_nothing; trivial.
-  destruct blk2; simpl in *.
-  split;
-  apply refine_ret_ret_fst_Same; trivial;
-  apply Same_Same_set;
-  [|symmetry];
-  apply Lookup_Update_idem; auto;
-  try (apply allocations_functional; auto);
-  intros; destruct (N.eq_dec a a'); auto.
-Qed.
-*)
-
-Lemma simply_within : forall n m A (P Q : A),
-  0 < m -> Ifdec within n m n Then P Else Q = P.
-Proof. intros; decisions; auto; nomega. Qed.
-
-Corollary within_nothing : forall addr p, ~ within addr 0 p.
-Proof. nomega. Qed.
-
 Theorem buffer_cons_sound
         (r_o : list Word) (r_n : PS)
         (AbsR : ByteString_list_AbsR r_o r_n) :
@@ -335,16 +140,16 @@ Theorem buffer_cons_sound
     ByteString_list_AbsR (x :: r_o) r_n'.
 Proof.
   unfold buffer_cons; intros.
-  apply refine_computes_to_ret in H.
+  apply refine_computes_to in H.
   rewrite refineEquiv_If_Then_Else_Bind in H.
   apply refine_If_Then_Else_bool in H.
   destruct (0 <? psOffset r_n) eqn:Heqe.
-    apply refine_computes_to_ret in H.
+    apply computes_to_refine in H.
     {
       destruct_computations; simpl in *.
       destruct_AbsR AbsR; construct_AbsR.
       right; split; trivial; split; [nomega|].
-      split; intros; teardown;
+      split; intros;
       destruct_computations; tsubst;
       simpl; trivial.
       simplify_maps.
@@ -367,28 +172,24 @@ Proof.
   destruct (psLength r_n + alloc_quantum <=? psBufLen r_n) eqn:Heqe2;
   [| rewrite refineEquiv_If_Then_Else_Bind in H;
      destruct (0 <? psBufLen r_n) eqn:Heqe3; simpl in H ];
-  apply refine_computes_to_ret in H; revert H;
+  apply computes_to_refine in H; revert H;
   unfold make_room_by_shifting_up, make_room_by_growing_buffer,
          allocate_buffer, poke_at_offset;
   autorewrite with monad laws; simpl;
-  rewrite ?N.add_0_r;
-  unfold memcpy', alloc', free', poke';
-  rewrite refine_bind_dep_bind_ret; simpl;
-  repeat setoid_rewrite refine_bind_dep_bind_ret; simpl.
+  rewrite ?N.add_0_r.
   - simpl; intros; destruct_computations;
     destruct_AbsR AbsR; construct_AbsR;
     (right; split; [nomega|]; split; [nomega|]).
-    rewrite H0, N.add_0_r in *; clear H0.
+    rewrite H0, N.add_0_r in *; clear H0;
+    tsubst; simpl in *; subst.
     destruct (psLength r_n =? 0) eqn:Heqe.
       assert (psLength r_n = 0) by nomega.
       rewrite H in *; clear H.
-      destruct x1, x3; simpl.
       split; trivial.
       intros; simplify_maps.
       destruct i using N.peano_ind.
         left; nomega.
       nomega.
-    destruct x1, x3; simpl.
     split; trivial.
     intros; simplify_maps.
     destruct i using N.peano_ind.
@@ -403,21 +204,11 @@ Proof.
       apply H4; trivial.
       nomega.
     nomega.
-  - simpl; intros;
-    apply Bind_dep_inv in H;
-    destruct H as [? [x1 ?]];
-    assert (fromADT HeapSpec (fst x0))
-      by (eapply alloc_fromADT; eauto;
-          [ exact (proj2_sig (psHeap r_n))
-          | simpl; apply refine_computes_to_ret; apply x1 ]).
-    simpl; intros; destruct_computations;
+  - simpl; intros; destruct_computations;
     destruct_AbsR AbsR; construct_AbsR;
     (right; split; [nomega|]; split; [nomega|]).
-    rewrite H0, N.add_0_r in *; simpl in *; clear H0.
-    apply Bind_inv in x1; destruct x1 as [? [? ?]].
-    apply Pick_inv in H0; simpl in *.
-    destruct H5; simpl in *.
-    destruct_computations; simpl in *; tsubst.
+    rewrite H0, N.add_0_r in *; clear H0;
+    tsubst; simpl in *.
     split.
       simplify_maps.
       split.
@@ -431,9 +222,9 @@ Proof.
     right; split; [nomega|].
     rewrite N2Nat.inj_succ in *; simpl.
     apply copy_bytes_mapsto.
-    destruct (within_bool (x1 + 1) (psLength r_n)
-                          (x1 + N.succ i)) eqn:Heqe1; simpl.
-      replace (x1 + N.succ i - (x1 + 1) + psBuffer r_n)
+    destruct (within_bool (x0 + 1) (psLength r_n)
+                          (x0 + N.succ i)) eqn:Heqe1; simpl.
+      replace (x0 + N.succ i - (x0 + 1) + psBuffer r_n)
          with (psBuffer r_n + i) by nomega.
       apply H4; trivial.
       nomega.
@@ -441,8 +232,8 @@ Proof.
   - simpl; intros; destruct_computations;
     destruct_AbsR AbsR; construct_AbsR;
     (right; split; [nomega|]; split; [nomega|]).
-    destruct_computations; simpl in *.
-    rewrite H3, ?N.add_0_r in *; simpl.
+    destruct_computations; tsubst; simpl in *.
+    rewrite ?N.add_0_r in *; simpl.
     split.
       simplify_maps.
     intros.
@@ -463,16 +254,12 @@ Theorem buffer_uncons_sound : forall r_o r_n a,
                              end) (fst a).
 Proof.
   unfold buffer_uncons; intros.
-  apply refine_computes_to_ret in H0.
+  apply refine_computes_to in H0.
   apply refine_If_Then_Else_bool in H0.
   destruct (0 <? psLength r_n) eqn:Heqe.
     revert H0.
-    unfold peek'.
-    rewrite refine_bind_dep_bind_ret; simpl.
-    rewrite refine_bind_dep_ignore.
-    unfold peek.
     autorewrite with monad laws; simpl; intros.
-    apply refine_computes_to_ret in H0.
+    apply computes_to_refine in H0.
     destruct_computations; simpl.
     destruct_AbsR H; construct_AbsR;
     destruct x; try destruct p; simpl in *;
@@ -497,7 +284,7 @@ Proof.
     rewrite N2Nat.inj_succ in *; simpl.
     rewrite N2Nat.inj_add, Nat.add_1_r.
     assumption.
-  apply refine_computes_to_ret in H0.
+  apply computes_to_refine in H0.
   destruct_computations.
   destruct_AbsR H; construct_AbsR;
   destruct r_o; simpl in *; auto; try nomega.
@@ -514,26 +301,22 @@ Theorem buffer_uncons_impl : forall r_o r_n a,
                end.
 Proof.
   unfold buffer_uncons; intros.
-  apply refine_computes_to_ret in H0.
+  apply refine_computes_to in H0.
   apply refine_If_Then_Else_bool in H0.
   destruct (0 <? psLength r_n) eqn:Heqe.
     revert H0.
-    unfold peek'.
-    rewrite refine_bind_dep_bind_ret; simpl.
-    rewrite refine_bind_dep_ignore.
-    unfold peek.
     autorewrite with monad laws; simpl; intros.
-    apply refine_computes_to_ret in H0.
+    apply computes_to_refine in H0.
     destruct_computations.
     destruct_AbsR H; simpl;
     destruct r_o; simpl in *; try nomega.
-    f_equal.
+    f_equal; tsubst.
     apply H0.
     replace (psBuffer r_n + psOffset r_n)
        with (psBuffer r_n + psOffset r_n + 0) by nomega.
     apply H4; trivial.
     nomega.
-  apply refine_computes_to_ret in H0.
+  apply computes_to_refine in H0.
   apply Return_inv in H0.
   destruct a; tsubst; simpl in *.
   destruct r_o; simpl in *;
@@ -546,7 +329,7 @@ Qed.
 
 Section Refined.
 
-Variable heap : Rep HSpec.
+Variable heap : Rep HeapSpec.
 
 Lemma ByteStringHeap  : { adt : _ & refineADT ByteStringSpec adt }.
 Proof.
