attic/Tactics.v
@@ -1,0 +1,234 @@
+Require Export
+  Coq.Sets.Constructive_sets
+  Coq.Sets.Powerset_facts.
+
+Require Import Fiat.ADT.
+
+Ltac single_reduction :=
+  match goal with
+  | [ |- Strict_Included _ _ _ ] => constructor
+  | [ |- Included _ _ _ ] =>
+    let x := fresh "x" in
+    let Hx := fresh "Hx" in
+    intros x Hx
+  | [ H : _ /\ _ |- _ ] => destruct H
+  | [ |- _ /\ _ ] => split
+  | [ H : _ * _ |- _ ] => destruct H
+  | [ |- _ * _ ] => split
+  | [ H : Ensembles.In _ _ _ |- _ ] => inv H
+  | [ H : Ensembles.In _ _ _ |- _ ] => rewrite H in *
+  | [ |- Ensembles.In _ _ _ ] => constructor
+  | [ |- Ensembles.In _ (Bind _ (fun x => ret _)) _ ] => eexists
+  | [ |- Ensembles.In _ _ _ ] => eexists
+  | [ H : forall x : ?T, Some ?X = Some x -> _ |- _ ] =>
+    specialize (H X eq_refl)
+  | [ |- ret ?C ↝ ?V -> _ ] =>
+    let H := fresh "H" in intro H; apply Return_inv in H; simpl in H; inv H
+  | [ |- Bind ?C ?F ↝ ?V -> _ ] =>
+    let H := fresh "H" in intro H; apply Bind_inv in H; simpl in H; inv H
+  | [ |- Pick ?S ↝ ?V -> _ ] =>
+    let H := fresh "H" in intro H; apply Pick_inv in H; simpl in H; inv H
+  | [ H : ret ?C ↝ ?V     |- _ ] => apply Return_inv in H
+  | [ H : Bind ?C ?F ↝ ?V |- _ ] => apply Bind_inv in H
+  | [ H : Pick ?S ↝ ?V    |- _ ] => apply Pick_inv in H
+  | [ |- ret ?C ↝ ?V ]           => apply ReturnComputes
+  | [ |- Bind ?C ?F ↝ ?V ]       => apply BindComputes
+  | [ |- Pick ?S ↝ ?V ]          => apply PickComputes
+  | [ |- context [If_Opt_Then_Else ?V ?T ?E] ] => destruct V
+  (* | [ |- context [Ifdec_Then_Else ?P ?T ?E] ]  => unfold Ifdec_Then_Else *)
+  end.
+
+Ltac simplify_ensembles :=
+  repeat (single_reduction; simpl; destruct_ex);
+  try solve [ intuition | constructor ].
+
+Require Import
+  Fiat.ADT
+  Fiat.ADTNotation.
+
+Tactic Notation "refine" "method" constr(name) :=
+  match goal with
+    | [ _ : constructorType ?A (consDom {| consID := name
+                                         ; consDom := _ |}) |- _ ] =>
+      idtac "Constructor"
+    | [ _ : methodType ?A (methDom {| methID := name
+                                    ; methDom := _
+                                    ; methCod := _ |})  _ |- _ ] =>
+      idtac "Method"
+    | _ =>
+      fail "Incorrect method name"
+  end.
+
+Require Import
+  Coq.Sets.Ensembles
+  Fiat.ADT
+  Fiat.ADTNotation
+  FunctionalExtensionality.
+
+Axiom prop_ext : forall (P Q : Prop), (P <-> Q) -> P = Q.
+
+Ltac shatter :=
+  unfold id in *;
+  repeat
+    match goal with
+    | [ H : and _ _            |- _                 ] => destruct H
+    | [ H : Bind _ _ _         |- _                 ] => destruct H
+    | [ H : In _ _ _           |- _                 ] => destruct H
+    | [ H : Datatypes.prod _ _ |- _                 ] => destruct H
+    | [                        |- and _ _           ] => split
+    | [                        |- Bind _ _ _        ] => eexists
+    | [                        |- In _ _ _          ] => constructor
+    | [                        |- In _ _ _          ] => solve [ eauto ]
+    | [                        |- In _ (Bind _ _) _ ] => eexists
+    | [                        |- In _ _ _          ] => econstructor
+    end;
+  simpl in *.
+
+(** Until the FunctorLaws are expressed in terms of some arbitrary
+    equivalence, we need to use functional and propositional
+    extensionality. *)
+
+Ltac simplify_comp :=
+  repeat let x := fresh "x" in extensionality x;
+  try (apply prop_ext; split; intros);
+  repeat shatter;
+  try constructor; eauto.
+
+Ltac zoom T :=
+  let Ty := type of T in
+  let U := fresh "U" in evar (U : Ty);
+  let H := fresh "H" in assert (T = U) as H;
+    [ subst U | setoid_rewrite H; clear H; unfold U; clear U ].
+
+Ltac shift tac := etransitivity; [apply tac|].
+
+Lemma surjective_pairing_r : forall A B (x : A * B),
+  (fst x, snd x) = x.
+Proof.
+  intros.
+  destruct x; reflexivity.
+Qed.
+
+Ltac adjust term :=
+  let T := constr:term in
+  assert { T' : _ & T = T'} as T'; [eexists| apply (projT1 T')].
+
+Require Import
+  Fiat.ADTRefinement
+  Fiat.ADTRefinement.BuildADTRefinements.
+
+Tactic Notation "refine" "method" constr(name) :=
+  match goal with
+    | [ _ : constructorType ?A (consDom {| consID := name
+                                         ; consDom := _ |}) |- _ ] =>
+      idtac "Constructor"
+    | [ _ : methodType ?A (methDom {| methID := name
+                                    ; methDom := _
+                                    ; methCod := _ |})  _ |- _ ] =>
+      idtac "Method"
+    | _ =>
+      fail "Incorrect method name"
+  end.
+
+Ltac finish_concrete :=
+  match goal with
+  | [ |- context[Pick _] ] => idtac
+  | _ => finish honing
+  end.
+
+Ltac simplify_ADT :=
+  try simplify with monad laws; simpl;
+  try match goal with
+    [ H : _ = _ |- _ ] =>
+    rewrite H; clear H
+  end;
+  try refine pick eq;
+  try refine pick val tt; try tauto;
+  try simplify with monad laws;
+  try finish_concrete.
+
+Lemma refineEquiv_If_Then_Else_Bind :
+  forall (A B : Type) (i : bool) (t e : Comp A) (b : A -> Comp B),
+    refineEquiv (a <- If i Then t Else e; b a)
+                (If i Then a <- t; b a Else (a <- e; b a)).
+Proof. split; intros; destruct i; reflexivity. Qed.
+
+Theorem refine_If_Then_Else_bool :
+  forall (b : bool) A cpst cpse (res : Comp A),
+    (if b then refine cpst res else refine cpse res)
+      <-> refine (If b Then cpst Else cpse) res.
+Proof. split; intros; destruct b; auto. Qed.
+
+Lemma refineEquiv_Ifopt_Then_Else_Bind :
+  forall A B T (i : option T) (t : T -> Comp A) (e : Comp A) (b : A -> Comp B),
+    refineEquiv (a <- Ifopt i as p Then t p Else e; b a)
+                (Ifopt i as p Then a <- t p; b a Else (a <- e; b a)).
+Proof. split; intros; destruct i; reflexivity. Qed.
+
+Require Import ByteString.Decidable.
+
+Lemma refineEquiv_Ifdec_Then_Else_Bind :
+  forall A B `{Decidable i} (t e : Comp A) (b : A -> Comp B),
+    refineEquiv (a <- Ifdec i Then t Else e; b a)
+                (Ifdec i Then a <- t; b a Else (a <- e; b a)).
+Proof.
+  intros.
+  destruct H.
+  unfold Ifdec_Then_Else; simpl.
+  destruct Decidable_witness; reflexivity.
+Qed.
+
+Lemma refine_ret_ret_eq : forall A (a b : A),
+  refine (ret a) (ret b) <-> a = b.
+Proof.
+  split; intros.
+    specialize (H b (ReturnComputes b)).
+    apply Return_inv; assumption.
+  destruct H.
+  reflexivity.
+Qed.
+
+Require Import ByteString.TupleEnsembles.
+
+Lemma refine_ret_ret_Same : forall A B (a b : EMap A B),
+  refine (ret a) (ret b) <-> Same a b.
+Proof.
+  split; intros.
+    specialize (H b (ReturnComputes b)).
+    destruct H.
+    reflexivity.
+  f_equiv.
+  apply Extensionality_Ensembles, Same_Same_set.
+  assumption.
+Qed.
+
+Lemma refine_ret_ret_fst_Same : forall A (x z : Comp A) B (y w : B),
+  Same_set _ x z -> y = w -> refine (ret (x, y)) (ret (z, w)).
+Proof.
+  intros; subst; f_equiv; f_equal.
+  apply Extensionality_Ensembles; assumption.
+Qed.
+
+Ltac breakdown :=
+  match goal with
+  | [ H : IF _ then _ else _ |- _ ] => destruct H
+  | [ H : _ /\ _             |- _ ] => destruct H
+  | [ H : _ \/ _             |- _ ] => destruct H
+  | [ H : _ * _              |- _ ] => destruct H
+  | [ H : exists _, _        |- _ ] => destruct H
+  | [ H : @sig _ _           |- _ ] => destruct H
+  | [ H : @sig2 _ _ _        |- _ ] => destruct H
+  | [ H : @sigT _ _          |- _ ] => destruct H
+  | [ H : @sigT2 _ _ _       |- _ ] => destruct H
+  | [ H : bool               |- _ ] => destruct H
+  | [ H : option _           |- _ ] => destruct H
+  | [ H : sum _ _            |- _ ] => destruct H
+  | [ H : sumor _ _          |- _ ] => destruct H
+  | [ H : sumbool _ _        |- _ ] => destruct H
+
+  | [ H : forall x, Some ?X = Some x -> _  |- _ ] => specialize (H X eq_refl)
+  | [ H : forall x y, Some (?X, ?Y) = Some (x, y) -> _  |- _ ] =>
+    specialize (H X Y eq_refl)
+
+  | [ H1 : ?X = true, H2 : ?X = false |- _ ] => rewrite H1 in H2; discriminate
+  end.
