attic/Within.v
@@ -15,6 +15,33 @@ Include X.
 
 Module Import Block := MemoryBlockC M.
 
+Local Open Scope lsignature_scope.
+
+Lemma within_AbsR :
+  within [R N.eq ==> N.eq ==> N.eq ==> boolR] within_bool.
+Proof.
+  intros.
+  relational; unfold Basics.compose, negb; split; intros.
+    rewrite H, H0, H1 in H2.
+    decisions; auto; nomega.
+  rewrite <- H, <- H0, <- H1 in H2.
+  decisions; auto; nomega.
+Qed.
+
+Lemma not_within_AbsR : forall b l,
+  (Basics.compose not (within b l))
+    [R N.eq ==> boolR] (Basics.compose negb (within_bool b l)).
+Proof.
+  intros.
+  relational; unfold Basics.compose, negb; split; intros.
+    rewrite H in H0.
+    decisions; auto; nomega.
+  rewrite <- H in H0.
+  decisions; auto.
+    discriminate.
+  nomega.
+Qed.
+
 Definition within_allocated_mem (n : N) :=
   fun (addr : M.key) (blk : MemoryBlockC) => addr + memCSize blk <=? n.
 Arguments within_allocated_mem n addr blk /.
