src/Fiat.v
@@ -1,0 +1,98 @@
+Require Export
+  Fiat.ADT
+  Fiat.ADTNotation
+  Fiat.ADTRefinement
+  Fiat.ADTRefinement.BuildADTRefinements
+  ByteString.ADTInduction.
+
+Tactic Notation "refine" "method" constr(name) :=
+  match goal with
+    | [ _ : constructorType ?A (consDom {| consID := name
+                                         ; consDom := _ |}) |- _ ] =>
+      idtac
+    | [ _ : methodType ?A (methDom {| methID := name
+                                    ; methDom := _
+                                    ; methCod := _ |})  _ |- _ ] =>
+      idtac
+    | _ =>
+      fail "Incorrect method name"
+  end.
+
+Ltac destruct_computations :=
+  repeat match goal with
+  | [ H : computes_to (Bind _ _) _     |- _ ] =>
+    let H0 := fresh "H0" in
+    apply Bind_inv in H; destruct H as [? [? H0]]
+  | [ H : computes_to (Pick _) _       |- _ ] =>
+    apply Pick_inv in H
+  | [ H : computes_to (Return _) _     |- _ ] =>
+    apply Return_inv in H; subst
+  | [ H : computes_to _ _ |- _ ] =>
+    let H0 := fresh "H0" in
+    first [ apply Bind_inv in H; destruct H as [? [? H0]]
+          | apply Pick_inv in H
+          | apply Return_inv in H; subst ]
+  end.
+
+Corollary refine_computes_to {A} {c : Comp A} {v} : c ↝ v -> refine c (ret v).
+Proof. intros ?? H0; destruct H0; assumption. Qed.
+
+Corollary computes_to_refine {A} {c : Comp A} {v} : refine c (ret v) -> c ↝ v.
+Proof. intuition. Qed.
+
+Corollary refine_pick_ret : forall A x,
+  refine {a : A | ret x ↝ a} (ret x).
+Proof. intuition. Qed.
+
+Corollary refine_inv : forall A old new,
+  refine old new -> forall x : A, new ↝ x -> old ↝ x.
+Proof. trivial. Qed.
+
+Lemma refineEquiv_If_Then_Else_Bind :
+  forall (A B : Type) (i : bool) (t e : Comp A) (b : A -> Comp B),
+    refineEquiv (a <- If i Then t Else e; b a)
+                (If i Then a <- t; b a Else (a <- e; b a)).
+Proof. split; intros; destruct i; reflexivity. Qed.
+
+Theorem refine_If_Then_Else_bool :
+  forall (b : bool) A cpst cpse (res : Comp A),
+    (if b then refine cpst res else refine cpse res)
+      <-> refine (If b Then cpst Else cpse) res.
+Proof. split; intros; destruct b; auto. Qed.
+
+Lemma fst_match_list :
+  forall A (xs : list A) B z C z'
+         (f : A -> list A -> B) (f' : A -> list A -> C),
+    fst match xs with
+        | List.nil => (z, z')
+        | List.cons x xs => (f x xs, f' x xs)
+        end = match xs with
+              | List.nil => z
+              | List.cons x xs => f x xs
+              end.
+Proof. induction xs; auto. Qed.
+
+Lemma snd_match_list :
+  forall A (xs : list A) B z C z'
+         (f : A -> list A -> B) (f' : A -> list A -> C),
+    snd match xs with
+        | List.nil => (z, z')
+        | List.cons x xs => (f x xs, f' x xs)
+        end = match xs with
+              | List.nil => z'
+              | List.cons x xs => f' x xs
+              end.
+Proof. induction xs; auto. Qed.
+
+Lemma If_Then_Else_fst : forall p A B (a b : A * B),
+  fst (If p Then a Else b) = If p Then (fst a) Else (fst b).
+Proof. intros; destruct p; trivial. Qed.
+
+Lemma If_Then_Else_snd : forall p A B (a b : A * B),
+  snd (If p Then a Else b) = If p Then (snd a) Else (snd b).
+Proof. intros; destruct p; trivial. Qed.
+
+Lemma If_Then_Else_pair : forall p A (a b : A) B (c d : B),
+  (If p Then a Else b, If p Then c Else d)
+    = If p Then (a, c) Else (b, d).
+Proof. intros; destruct p; trivial. Qed.
