src/FromADT.v
@@ -1,15 +1,8 @@
 Require Import
-  Fiat.ADT
-  Fiat.ADTNotation
-  ByteString.ADTInduction
-  ByteString.LibExt.
+  ByteString.Fiat
+  ByteString.ADTInduction.
 
-Require Import
-  Fiat.ADTRefinement
-  Fiat.ADTRefinement.BuildADTRefinements.
-
-Require Import
-  ByteString.BindDep.
+Generalizable All Variables.
 
 Definition fromADTConstructor'
            {dSig : DecoratedADTSig}
@@ -28,22 +21,8 @@ Notation fromCons adt idx :=
   (fromADTConstructor' adt (fun idx => ibound (indexb idx))
                            {| bindex := idx |}).
 
-Lemma refine_computes_to {A} {c : Comp A} {v} :
-  c ↝ v -> refine c (ret v).
-Proof.
-  intros.
-  intros ??.
-  inv H0.
-  exact H.
-Qed.
-
-Lemma computes_to_refine {A} {c : Comp A} {v} :
-  refine c (ret v) -> c ↝ v.
-Proof. intros; exact (H _ (ReturnComputes _)). Qed.
-
 Tactic Notation "check" "constructor" constr(t) :=
-  simpl; intros;
-  apply t;
+  simpl; intros; apply t;
   repeat match goal with
     | [ H : refine _ (ret _) |- _ ] => apply computes_to_refine in H
     | [ |- fromConstructor _ _ _ ] => eexists
@@ -81,51 +60,151 @@ Tactic Notation "check" "method" constr(t) :=
 
 Lemma refine_constructor_fromADT
       A (c : Comp (A)) (P : A -> Prop)
-      (f : forall v : A, refine c (ret v) -> P v) :
-   refine (r_o' <- c;
-           {r_n0 : {r : A | P r} | r_o' = ` r_n0})
-          (`(r_o' | H) <- c;
-           ret (exist _ r_o' (f r_o' H))).
+      (f : forall v : A, c ↝ v -> P v) :
+  refine (r_o' <- c; {r_n0 : {r : A | P r} | r_o' = ` r_n0})
+         { r_n0 : { r : A | P r } | c ↝ ` r_n0 }.
 Proof.
-  intros x?.
-  destruct H.
-  exists x0.
-  destruct H.
-  split; trivial.
-  destruct i.
-  esplit.
-Qed.
-
-Lemma refine_method_fromADT
-      A B (c : Comp (A * B)) (P : A -> Prop)
-      (f : forall v : A * B, refine c (ret v) -> P (fst v)) :
-   refine (r_o' <- c;
-           r_n' <- {r_n0 : {r : A | P r} | fst r_o' = ` r_n0};
-           ret (r_n', snd r_o'))
-          (`(r_o' | H) <- c;
-           ret (exist _ (fst r_o') (f r_o' H),
-                snd r_o')).
-Proof.
-  intros x?.
-  destruct H.
-  exists x0.
-  destruct H.
-  split; trivial.
-  destruct i.
-  esplit; split.
-    Focus 2.
-    constructor.
-  constructor.
+  intros x ?.
+  apply Pick_inv in H.
+  apply BindComputes with (a:=` x); trivial.
+  apply PickComputes.
+  reflexivity.
 Qed.
 
 Ltac resolve_constructor m H0 :=
   subst; subst_evars;
   etransitivity;
-  [ apply (refine_constructor_fromADT _ (c:=m) H0)
+  [ apply refine_constructor_fromADT;
+    intros ??; apply H0; assumption
   | finish honing].
+
+Lemma refine_method_fromADT
+      A B (c : Comp (A * B)) (P : A -> Prop)
+      (f : forall v : A * B, c ↝ v -> P (fst v)) :
+   refine (r_o' <- c;
+           r_n' <- {r_n0 : {r : A | P r} | fst r_o' = ` r_n0};
+           ret (r_n', snd r_o'))
+          { r_n0 : { r : A | P r } * B | c ↝ (` (fst r_n0), snd r_n0) }.
+Proof.
+  intros [x b] ?.
+  apply Pick_inv in H; simpl in H.
+  apply BindComputes with (a:=(` x, b)); trivial.
+  simpl.
+  apply BindComputes with (a:=x); trivial.
+  apply PickComputes.
+  reflexivity.
+Qed.
 
 Ltac resolve_method r_n m H0 :=
   subst; subst_evars;
   etransitivity;
-  [ apply (refine_method_fromADT _ (c:=m) H0)
+  [ apply refine_method_fromADT;
+    intros ??; apply H0; assumption
   | finish honing].
+
+Lemma refine_strip_dependency :
+  forall A (P : A -> Prop) x B (k : _ -> Comp B),
+    P x ->
+    refine (a <- {r_n0 : {r : A | P r} | ret x ↝ ` r_n0}; k (` a))
+           (a <- {r_n0 : A | ret x ↝ r_n0}; k a).
+Proof.
+  intros; intros ??.
+  apply Bind_inv in H0; destruct H0 as [? [? ?]].
+  apply Pick_inv in H0; destruct H0.
+  eapply BindComputes with (a:=exist _ x H); eauto.
+Qed.
+
+Ltac strip_dependency_constructor :=
+  let x := fresh "x" in
+  let H := fresh "H" in
+  match goal with
+  | [ |- refine (_ <- _; _) _ ] =>
+    eapply refine_under_bind_helper; intros x H;
+    [ exact H
+    | let H := fresh "H" in
+      intro H;
+      pattern (` x);
+      match goal with
+      | [ |- (fun h : ?T => refine ?X ?Y) (` x) ] =>
+        change (refine ((fun h : T => X) (` x)) Y)
+      end;
+      exact H
+    | rewrite refine_strip_dependency ]
+  end;
+  revert H;
+  revert x;
+  try apply refine_inv.
+
+Lemma refine_strip_dependency_pair :
+  forall A (P : A -> Prop) B c C (k : A -> B -> Comp C),
+    (forall v, c ↝ v -> P (fst v)) ->
+    refine (a <- {r_n0 : {r : A | P r} * B
+                 | c ↝ (` (fst r_n0), snd r_n0)};
+            k (` (fst a)) (snd a))
+           (a <- {r_n0 : A * B | c ↝ r_n0};
+            k (fst a) (snd a)).
+Proof.
+  intros; intros ??.
+  apply Bind_inv in H0; destruct H0 as [? [? ?]].
+  apply Pick_inv in H0.
+  apply BindComputes with (a:=(exist _ (fst x) (H _ H0), snd x)); eauto.
+  apply PickComputes; simpl.
+  rewrite <- surjective_pairing.
+  assumption.
+Qed.
+
+Ltac strip_dependency_method :=
+  let x := fresh "x" in
+  let H := fresh "H" in
+  match goal with
+  | [ |- refine (_ <- _; _) _ ] =>
+    eapply refine_under_bind_helper; intros x H;
+    [ exact H
+    | let H := fresh "H" in
+      intro H;
+      pattern (snd x);
+      pattern (` (fst x));
+      match goal with
+      | [ |- (fun h : ?T => (fun p : ?U => refine ?X ?Y) (snd x))
+               (` (fst x)) ] =>
+        change (refine ((fun (h : T) (p : U) => X) (` (fst x)) (snd x)) Y)
+      end;
+      exact H
+    | rewrite refine_strip_dependency_pair ]
+  end;
+  revert H;
+  revert x;
+  try apply refine_inv.
+
+Lemma refine_dependency A (X : Comp A) B (f : B -> A) C (k : B -> Comp C) :
+  refine (a <- {a : B | X ↝ f a}; k a)
+         (x <- X; a <- {a : B | ret x ↝ f a}; k a).
+Proof.
+  intros ??.
+  apply Bind_inv in H; destruct H as [? [? ?]].
+  apply computes_to_refine.
+  apply Bind_inv in H0; destruct H0 as [? [? ?]].
+  refine pick val x0; simpl; trivial.
+    simplify with monad laws.
+    apply refine_computes_to.
+    assumption.
+  apply Pick_inv in H0; destruct H0.
+  assumption.
+Qed.
+
+Ltac remove_dependency HA :=
+  first [ strip_dependency_constructor;
+          [| intros; apply HA; simpl ];
+          rewrite refine_pick_ret; simpl
+        | strip_dependency_method;
+          [ rewrite refine_dependency;
+            setoid_rewrite refine_pick_ret; simpl
+          | let H := fresh "H" in
+            intros ? ? ? H;
+            eapply HA; simpl;
+            [ match goal with
+                [ HR : { r : _ | _ r } |- _ ] =>
+                exact (proj2_sig HR)
+              end
+            | exact H ] ] ];
+  try simplify with monad laws; simpl.
